DY/Actions/Compromise.lean
@@ -1,0 +1,128 @@
+module
+
+public import DY.Trace
+public import DY.Bytes
+public import DY.Actions.PersistentGlobalState
+public import DY.Actions.ProtocolEvent
+public import DY.Actions.Network
+public import DY.Comparse
+import DY.Step
+
+namespace DY.Compromise
+
+public
+structure CompromiseEvent (StateT: Type) where
+  state: StateT
+
+public
+def compromise
+  (StateT: Type)
+  [BytesFunctor]
+  [Comparse.ParseableSerializeable StateT]
+  [ExecTraceTypes]
+  [ExecTraceTypes.Has Network.ExecEntryT]
+  [ExecTraceTypes.Has (PersistentGlobalState.ExecEntryT StateT)]
+  [ExecTraceTypes.Has (ProtocolEvent.ExecEntryT (CompromiseEvent StateT))]
+  (i: Nat)
+  : Traceful Nat
+:= do
+  let state: StateT ← PersistentGlobalState.getGlobalState i
+  ProtocolEvent.logEvent ({ state }: CompromiseEvent StateT)
+  Network.sendMessage (Comparse.ParseableSerializeable.serialize state)
+
+public
+def GlobalStateCompromised
+  {StateT: Type}
+  [ExecTraceTypes] [ExecTraceTypes.Has (ProtocolEvent.ExecEntryT (CompromiseEvent StateT))]
+  (state: StateT)
+  (tr: ExecTrace)
+  : Prop
+:=
+  tr.EventLogged ({ state }: CompromiseEvent StateT)
+
+public
+theorem GlobalStateCompromised_le
+  {StateT: Type}
+  [ExecTraceTypes] [ExecTraceTypes.Has (ProtocolEvent.ExecEntryT (CompromiseEvent StateT))]
+  (state: StateT)
+  (tr1 tr2: ExecTrace)
+  : tr1 ≤ tr2 →
+    GlobalStateCompromised state tr1 →
+    GlobalStateCompromised state tr2
+:= by
+  simp [GlobalStateCompromised]
+  grind
+
+grind_pattern GlobalStateCompromised_le => tr1 ≤ tr2, GlobalStateCompromised state tr1
+
+public
+def label
+  {StateT: Type}
+  [ExecTraceTypes] [ExecTraceTypes.Has (ProtocolEvent.ExecEntryT (CompromiseEvent StateT))]
+  (state: StateT)
+:=
+  ProtocolEvent.label ({ state }: CompromiseEvent StateT)
+
+public
+theorem label_isCorrupt
+  {StateT: Type}
+  [ExecTraceTypes] [ExecTraceTypes.Has (ProtocolEvent.ExecEntryT (CompromiseEvent StateT))]
+  (state: StateT)
+  (tr: ExecTrace)
+  : (label state).isCorrupt tr = GlobalStateCompromised state tr
+:= by
+  grind [label, GlobalStateCompromised]
+
+grind_pattern label_isCorrupt => (label state).isCorrupt tr
+
+public
+class CompromisableStateInv
+  (StateT: Type)
+  [TraceTypes]
+  [BytesFunctor] [BytesInvariants]
+  [Comparse.ParseableSerializeable StateT]
+  [PersistentGlobalState.GlobalStateInv StateT]
+  [ExecTraceTypes.Has (ProtocolEvent.ExecEntryT (CompromiseEvent StateT))]
+where
+  invariant_implies_KnowableBy:
+    ∀ (state: StateT) tr,
+      PersistentGlobalState.GlobalStateInv.invariant state tr →
+      Comparse.isWellFormed (Bytes.KnowableBy (label state)) state tr
+
+public
+instance
+  {StateT: Type}
+  [TraceTypes]
+  : ProtocolEvent.EventInv (CompromiseEvent StateT)
+where
+  invariant _ _ := True
+
+@[instance]
+public
+theorem compromise.spec
+  {StateT: Type}
+  [TraceInvariant]
+  [BytesFunctor] [BytesInvariants] [BytesInvariantsProofs]
+  [PersistentGlobalState.GlobalStateInv StateT]
+  [Comparse.ParseableSerializeable StateT]
+  [TraceTypes.Has Network.ProofEntryFunc] [TraceInvariant.Has Network.Invariant]
+  [TraceTypes.Has (PersistentGlobalState.ProofEntryFunc StateT)] [TraceInvariant.Has (PersistentGlobalState.Invariant StateT)]
+  [TraceTypes.Has (ProtocolEvent.ProofEntryFunc (CompromiseEvent StateT))] [TraceInvariant.Has (ProtocolEvent.Invariant (CompromiseEvent StateT))]
+  [CompromisableStateInv StateT]
+  (i: Nat)
+  : HoareTriple
+    (compromise StateT i)
+    (fun _ => True)
+    (fun _ _ => True)
+:= by
+  apply HoareTriple.mk
+  unfold compromise
+  step
+  step by simp [ProtocolEvent.EventInv.invariant]
+  step by
+    have := CompromisableStateInv.invariant_implies_KnowableBy state tr
+    have : (label state).isCorrupt tr.erase := by simp_all [label, ProtocolEvent.label_isCorrupt]
+    grind [Comparse.isWellFormed, canFlowTrans]
+  trivial
+
+end DY.Compromise
