DY/Actions/PersistentGlobalState.lean
@@ -1,0 +1,103 @@
+module
+
+public import DY.Trace
+public import DY.Bytes
+import DY.Step.Init
+
+namespace DY.PersistentGlobalState
+
+public
+structure ExecEntryT (StateT: Type) where
+  st: StateT
+
+public
+def baseAttackerKnowledge [BytesFunctor] [ExecTraceTypes] (StateT: Type): EntryBaseAttackerKnowledge (ExecEntryT StateT) where
+  attackerKnows _ _ _ := False
+
+public
+abbrev ProofEntryT (StateT: Type) := ExecEntryT StateT
+
+public
+def ProofEntryFunc (StateT: Type) := ProofEntryFun.default (ExecEntryT StateT)
+
+public
+class GlobalStateInv [TraceTypes] (StateT: Type) where
+  invariant: StateT → ProofTrace → Prop
+  invariant_later: ∀ st tr1 tr2,
+    tr1 ≤ tr2 →
+    invariant st tr1 →
+    invariant st tr2
+
+grind_pattern GlobalStateInv.invariant_later => tr1 ≤ tr2, GlobalStateInv.invariant st tr1
+
+public
+def Invariant [TraceTypes] (StateT: Type) [GlobalStateInv StateT]: TraceEntryInvariant (ProofEntryFunc StateT) where
+  invariant tr entry :=
+    GlobalStateInv.invariant entry.st tr
+
+public
+theorem baseAttackerKnowledgeTheorem [TraceInvariant] [BytesFunctor] [BytesInvariants] (StateT: Type) [TraceTypes.Has (ProofEntryFunc StateT)] [GlobalStateInv StateT] [TraceInvariant.Has (Invariant StateT)]: EntryBaseAttackerKnowledgeTheorem (Invariant StateT) (baseAttackerKnowledge StateT) where
+  pf trBefore entry b := by
+    simp [baseAttackerKnowledge]
+
+public
+def storeGlobalState
+  {StateT: Type}
+  [ExecTraceTypes] [ExecTraceTypes.Has (ExecEntryT StateT)]
+  (st: StateT)
+  : Traceful Nat
+:= do
+  let entry: ExecEntryT StateT := { st }
+  appendEntry entry
+
+@[instance]
+public
+theorem storeGlobalState.spec
+  {StateT: Type}
+  [TraceInvariant]
+  [GlobalStateInv StateT]
+  [TraceTypes.Has (ProofEntryFunc StateT)] [TraceInvariant.Has (Invariant StateT)]
+  (st: StateT)
+  : HoareTriple
+    (storeGlobalState st)
+    (fun tr => GlobalStateInv.invariant st tr)
+    (fun _ _ => True)
+:= by
+  apply HoareTriple.mk
+  unfold storeGlobalState
+  dsimp only
+  step with ⟨ fun _ => ExecEntryT.mk st ⟩ by simp_all [ProofEntryFunc, Invariant]
+  trivial
+
+public
+def getGlobalState
+  {StateT: Type}
+  [ExecTraceTypes] [ExecTraceTypes.Has (ExecEntryT StateT)]
+  (i: Nat)
+  : Traceful StateT
+:= do
+  let e: ExecEntryT StateT ← getEntry i
+  return e.st
+
+@[instance]
+public
+theorem getGlobalState.spec
+  {StateT: Type}
+  [TraceInvariant]
+  [GlobalStateInv StateT]
+  [TraceTypes.Has (ProofEntryFunc StateT)] [TraceInvariant.Has (Invariant StateT)]
+  (i: Nat)
+  : HoareTriple
+    (getGlobalState i: Traceful StateT)
+    (fun _ => True)
+    (fun st tr => GlobalStateInv.invariant st tr)
+:= by
+  apply HoareTriple.mk
+  unfold getGlobalState
+  step
+  have: GlobalStateInv.invariant e.st tr := by simp_all [ProofEntryFunc, Invariant]; grind
+  rename_i h; clear h
+  step
+  grind
+
+end DY.PersistentGlobalState
