DY/Actions/PersistentLocalState.lean
@@ -1,0 +1,203 @@
+module
+
+public import DY.Trace
+public import DY.Bytes
+public import DY.Actions.PersistentGlobalState
+public import DY.Actions.Compromise
+import DY.Step.Init
+
+namespace DY.PersistentLocalState
+
+public
+abbrev Participant := String
+
+public
+structure LocalState (StateT: Type) where
+  participant: Participant
+  state: StateT
+
+public
+abbrev ExecEntryT (StateT: Type) := PersistentGlobalState.ExecEntryT (LocalState StateT)
+
+public
+def baseAttackerKnowledge [BytesFunctor] [ExecTraceTypes] (StateT: Type) := PersistentGlobalState.baseAttackerKnowledge (LocalState StateT)
+
+public
+def ProofEntryT (StateT: Type) := PersistentGlobalState.ProofEntryT (LocalState StateT)
+
+public
+abbrev ProofEntryFunc (StateT: Type) := PersistentGlobalState.ProofEntryFunc (LocalState StateT)
+
+public
+class LocalStateInv [TraceTypes] (StateT: Type) where
+  invariant: Participant → StateT → ProofTrace → Prop
+  invariant_later: ∀ p st tr1 tr2,
+    tr1 ≤ tr2 →
+    invariant p st tr1 →
+    invariant p st tr2
+
+grind_pattern LocalStateInv.invariant_later => tr1 ≤ tr2, LocalStateInv.invariant p st tr1
+
+public
+instance
+  [TraceTypes]
+  (StateT: Type) [LocalStateInv StateT]
+  : PersistentGlobalState.GlobalStateInv (LocalState StateT)
+where
+  invariant st tr := LocalStateInv.invariant st.participant st.state tr
+  invariant_later st tr1 tr2 := LocalStateInv.invariant_later st.participant st.state tr1 tr2
+
+public
+abbrev Invariant [TraceTypes] (StateT: Type) [LocalStateInv StateT] := PersistentGlobalState.Invariant (LocalState StateT)
+
+public
+def baseAttackerKnowledgeTheorem [TraceInvariant] [BytesFunctor] [BytesInvariants] (StateT: Type) [TraceTypes.Has (ProofEntryFunc StateT)] [LocalStateInv StateT] [TraceInvariant.Has (Invariant StateT)] := PersistentGlobalState.baseAttackerKnowledgeTheorem (LocalState StateT)
+
+public
+def storeLocalState
+  {StateT: Type}
+  [ExecTraceTypes] [ExecTraceTypes.Has (ExecEntryT StateT)]
+  (participant: Participant) (state: StateT)
+  : Traceful Nat
+:= do
+  PersistentGlobalState.storeGlobalState ({ participant, state }: LocalState StateT)
+
+@[instance]
+public
+theorem storeLocalState.spec
+  {StateT: Type}
+  [TraceInvariant]
+  [LocalStateInv StateT]
+  [TraceTypes.Has (ProofEntryFunc StateT)] [TraceInvariant.Has (Invariant StateT)]
+  (participant: Participant) (state: StateT)
+  : HoareTriple
+    (storeLocalState participant state)
+    (fun tr => LocalStateInv.invariant participant state tr)
+    (fun _ _ => True)
+:= by
+  apply HoareTriple.mk
+  unfold storeLocalState
+  step by simp_all [PersistentGlobalState.GlobalStateInv.invariant]
+  trivial
+
+public
+def getLocalState
+  {StateT: Type}
+  [ExecTraceTypes] [ExecTraceTypes.Has (ExecEntryT StateT)]
+  (participant: Participant) (i: Nat)
+  : Traceful StateT
+:= do
+  let st: LocalState StateT ← PersistentGlobalState.getGlobalState i
+  guard (st.participant = participant)
+  return st.state
+
+@[instance]
+public
+theorem getLocalState.spec
+  {StateT: Type}
+  [TraceInvariant]
+  [LocalStateInv StateT]
+  [TraceTypes.Has (ProofEntryFunc StateT)] [TraceInvariant.Has (Invariant StateT)]
+  (participant: Participant) (i: Nat)
+  : HoareTriple
+    (getLocalState participant i: Traceful StateT)
+    (fun _ => True)
+    (fun st tr => LocalStateInv.invariant participant st tr)
+:= by
+  apply HoareTriple.mk
+  unfold getLocalState
+  step
+  step
+  step
+  simp_all [PersistentGlobalState.GlobalStateInv.invariant]
+
+public
+def LocalStateCompromised
+  {StateT: Type}
+  [ExecTraceTypes] [ExecTraceTypes.Has (ProtocolEvent.ExecEntryT (Compromise.CompromiseEvent (LocalState StateT)))] -- ugh
+  (participant: Participant) (state: StateT)
+  (tr: ExecTrace)
+  : Prop
+:=
+  Compromise.GlobalStateCompromised ({ participant, state }: LocalState StateT) tr
+
+public
+theorem LocalStateCompromised_le
+  {StateT: Type}
+  [ExecTraceTypes] [ExecTraceTypes.Has (ProtocolEvent.ExecEntryT (Compromise.CompromiseEvent (LocalState StateT)))] -- ugh
+  (participant: Participant) (state: StateT)
+  (tr1 tr2: ExecTrace)
+  : tr1 ≤ tr2 →
+    LocalStateCompromised participant state tr1 →
+    LocalStateCompromised participant state tr2
+:= by
+  simp [LocalStateCompromised]
+  grind
+
+grind_pattern LocalStateCompromised_le => tr1 ≤ tr2, LocalStateCompromised participant state tr1
+
+public
+def label
+  {StateT: Type}
+  [ExecTraceTypes] [ExecTraceTypes.Has (ProtocolEvent.ExecEntryT (Compromise.CompromiseEvent (LocalState StateT)))] -- ugh
+  (participant: Participant) (state: StateT)
+:=
+  Compromise.label ({ participant, state }: LocalState StateT)
+
+public
+theorem label_isCorrupt
+  {StateT: Type}
+  [ExecTraceTypes] [ExecTraceTypes.Has (ProtocolEvent.ExecEntryT (Compromise.CompromiseEvent (LocalState StateT)))] -- ugh
+  (participant: Participant) (state: StateT)
+  (tr: ExecTrace)
+  : (label participant state).isCorrupt tr = LocalStateCompromised participant state tr
+:= by
+  grind [label, LocalStateCompromised]
+
+grind_pattern label_isCorrupt => (label participant state).isCorrupt tr
+
+public
+class CompromisableStateInv
+  (StateT: Type)
+  [TraceTypes]
+  [BytesFunctor] [BytesInvariants]
+  [Comparse.ParseableSerializeable StateT]
+  [LocalStateInv StateT]
+  [ExecTraceTypes.Has (ProtocolEvent.ExecEntryT (Compromise.CompromiseEvent (LocalState StateT)))] -- ugh
+where
+  invariant_implies_KnowableBy:
+    ∀ (participant: Participant) (state: StateT) tr,
+      LocalStateInv.invariant participant state tr →
+      Comparse.isWellFormed (Bytes.KnowableBy (label participant state)) state tr
+
+noncomputable
+instance
+  [BytesFunctor]
+  (StateT: Type)
+  [Comparse.ParseableSerializeable StateT]: Comparse.ParseableSerializeable (LocalState StateT) := Comparse.comparseMetaProgramExists
+
+axiom LocalState.isWellFormedLemma
+  [BytesFunctor]
+  {StateT: Type} [Comparse.ParseableSerializeable StateT]
+  (pre: Bytes → τ → Prop) [Comparse.BytesCompatible pre]
+  (x: LocalState StateT) (tr: τ):
+  Comparse.isWellFormed pre x tr = Comparse.isWellFormed pre x.state tr
+
+grind_pattern LocalState.isWellFormedLemma => Comparse.isWellFormed pre x tr
+
+instance
+  [TraceTypes] [BytesFunctor] [BytesInvariants]
+  (StateT: Type)
+  [Comparse.ParseableSerializeable StateT]
+  [LocalStateInv StateT]
+  [ExecTraceTypes.Has (ProtocolEvent.ExecEntryT (Compromise.CompromiseEvent (LocalState StateT)))] -- ugh
+  [CompromisableStateInv StateT]
+  : Compromise.CompromisableStateInv (LocalState StateT)
+where
+  invariant_implies_KnowableBy := by
+    intro { participant, state } tr
+    have := CompromisableStateInv.invariant_implies_KnowableBy participant state tr
+    simp [PersistentGlobalState.GlobalStateInv.invariant]
+    grind
+
+end DY.PersistentLocalState
